implement boolean within vector ops.

theories/Utils/BitVectors.v
@@ -16,6 +16,37 @@ Definition zeroByte : Byte :=
 Definition oneByte : Byte :=
   Vector.const true 8.
 
+Definition iffb (b1 b2 : bool) : bool :=
+  match b1, b2 with
+  | true, true => true
+  | false, true => false
+  | true, false => false 
+  | false, false => true
+  end.
+
+Theorem iffb_beq : forall {b1 b2}, (iffb b1 b2 = true) <-> b1 = b2.
+  intros [] []; split;
+  try reflexivity;
+  intro x; discriminate x.
+Qed.
+
+Definition bv_eq {n} (b1 b2 : Vector.t bool n) : bool.
+  apply (fun x : {b1 = b2} + {b1 <> b2} => if x then true else false).
+  apply (VectorEq.eq_dec bool iffb (@iffb_beq)).
+Defined.
+
+Definition bv_and {n} (b1 b2 : Vector.t bool n) : Vector.t bool n :=
+  Vector.map2 andb b1 b2.
+
+Definition bv_or {n} (b1 b2 : Vector.t bool n) : Vector.t bool n :=
+  Vector.map2 orb b1 b2.
+
+Definition bv_xor {n} (b1 b2 : Vector.t bool n) : Vector.t bool n :=
+  Vector.map2 xorb b1 b2.
+
+Definition bv_neg {n} (b : Vector.t bool n) : Vector.t bool n :=
+  Vector.map negb b.
+
 Definition bv_add : forall {n} (b1 b2 : Vector.t bool n), Vector.t bool n.
   intros n b1 b2.
   apply fin_bitvector; apply bitvector_fin in b1, b2.
@@ -24,6 +55,8 @@ Definition bv_add : forall {n} (b1 b2 : Vector.t bool n), Vector.t bool n.
   apply mod_upper_bound.
   lia.
 Defined.
+
+
 
 Definition bv_incr : forall {n}, Vector.t bool n -> nat -> Vector.t bool n.
   intros n b i.
